Adds alternative solver version

Unification_solver2.v
@@ -10,7 +10,7 @@ Import ListNotations.
 Definition unification_problem_is_bottom (u : unification_problem) : bool :=
   true.
 
-Inductive solver : Prop :=
+(*Inductive solver : Prop :=
   | Sbottom (u_p : unification_problem) (H : (unification_problem_is_bottom u_p) = true)
   | Ssolved (u_p : unification_problem) (H : (unification_problem_in_solved_form u_p) = true)
   | Sdelete (u_p u_p' : unification_problem)(H : ((term_in_unification_problem u_p term_eq) = true)) (H' : (remove_first_appearance_term_unification_problem u_p term_eq) = u_p')
@@ -30,5 +30,33 @@ Inductive solver : Type :=
   | Selimination (u : unification_problem)
   | Sconflict (u : unification_problem)
   | Soccurs_check (u : unification_problem).
+*)
 
-Fixpoint 
+Inductive solver : unification_problem -> Prop :=
+  | Sbottom : solver Ubottom
+  | Ssolved (u_p : unification_problem) (H : (unification_problem_in_solved_form u_p) = true) : solver u_p
+  | Sdelete (u_p u_p' : unification_problem)(H : ((term_in_unification_problem u_p term_eq) = true)) (H' : (remove_first_appearance_term_unification_problem u_p term_eq) = u_p')(H'' : solver u_p'): solver u_p
+  | Sdecompose (u_p u_p' : unification_problem)(H : ((term_in_unification_problem u_p is_decomposition_term_pair) = true)) (H': exists (tp : term_pair), (remove_and_replace_decomposition_unif_problem tp u_p) = u_p')(H'' : solver u_p'): solver u_p
+  | Sorientation (u_p u_p' : unification_problem) (H : ((term_in_unification_problem u_p is_orientation_term_pair) = true)) (H' : exists (tp : term_pair), (apply_orientation tp u_p) = u_p') (H'' : solver u_p'): solver u_p
+  | Selimination (u_p u_p' : unification_problem) (H : ((term_in_unification_problem u_p is_elimination_term_pair) = true)) (H' : exists (tp : term_pair), (elimination tp u_p) = u_p') (H'' : solver u_p'): solver u_p
+  | Sconflict (u_p u_p' : unification_problem) (H : ((term_in_unification_problem u_p is_conflict_term_pair) = true)) (H' : exists (tp : term_pair), (remove_conflict_term_pair tp u_p) = u_p') (H'' : solver u_p'): solver u_p
+  | Soccurs_check (u_p u_p' : unification_problem) (H : ((term_in_unification_problem u_p is_occurs_check_term_pair) = true)) (H' : exists (tp : term_pair), (occurs_check tp u_p) = u_p') (H'' : solver u_p'): solver u_p.
+
+Definition is_bottom (u : unification_problem) : bool :=
+  match u with
+  | Ubottom => true
+  | _ => false
+  end.
+
+
+Theorem is_solved_in_one_step : forall (u_p : unification_problem),
+  ((is_bottom u_p) = true) \/ ((unification_problem_in_solved_form u_p) = true) ->
+  solver u_p.
+Proof.
+  intros. destruct H.
+  - destruct u_p.
+    -- simpl in H. discriminate.
+    -- apply Sbottom.
+  - apply Ssolved. apply H.
+Qed. 
+
